src/program_proof/wal/heapspec_lib.v
@@ -1,0 +1,159 @@
+From Perennial.program_proof Require Import proof_prelude.
+From Perennial.program_proof Require Import wal.abstraction wal.transitions wal.lib.
+
+Definition no_updates (l: list update.t) a : Prop :=
+  forall u, u ∈ l -> u.(update.addr) ≠ a.
+
+Definition is_update (l: list update.t) a b : Prop :=
+  ∃ u, u ∈ l /\ u.(update.addr) = a /\ u.(update.b) = b.
+
+Theorem is_update_cons_eq: forall l a0,
+  is_update (a0 :: l) a0.(update.addr) a0.(update.b).
+Proof.
+  intros.
+  rewrite /is_update.
+  exists a0.
+  split; try auto.
+  apply elem_of_list_here.
+Qed.
+
+Theorem is_update_cons (l: list update.t) a b:
+  forall a0, is_update l a b -> is_update (a0 :: l) a b.
+Proof.
+  intros.
+  unfold is_update in *.
+  destruct H as [u [l1 H]].
+  intuition.
+  exists u.
+  split; auto.
+  apply elem_of_list_further; auto.
+Qed.
+
+Theorem latest_update_cons installed a:
+  forall bs,
+    bs ≠ [] ->
+    latest_update installed (a :: bs) = latest_update a bs.
+Proof.
+  intros.
+  unfold latest_update at 1.
+  simpl.
+  fold latest_update.
+  f_equal.
+Qed.
+
+Theorem latest_update_take_some bs v:
+  forall installed (pos: nat),
+    (installed :: bs) !! pos = Some v ->
+    latest_update installed (take pos bs) = v.
+Proof.
+  induction bs.
+  - intros.
+    rewrite firstn_nil.
+    simpl.
+    assert(pos = 0%nat).
+    {
+      apply lookup_lt_Some in H.
+      simpl in *.
+      word.
+    }
+    rewrite H0 in H.
+    simpl in *.
+    inversion H; auto.
+  - intros.
+    destruct (decide (pos = 0%nat)).
+    + rewrite e in H; simpl in *.
+      inversion H; auto.
+      rewrite e; simpl; auto.
+    +
+      assert (exists (pos':nat), pos = S pos').
+      {
+        exists (pred pos). lia.
+      }
+      destruct H0 as [pos' H0].
+      rewrite H0.
+      rewrite firstn_cons.
+      destruct (decide ((take pos' bs) = [])).
+      ++ simpl.
+         specialize (IHbs a pos').
+         apply IHbs.
+         rewrite lookup_cons_ne_0 in H; auto.
+         rewrite H0 in H; simpl in *; auto.
+      ++ rewrite latest_update_cons; auto.
+         {
+           specialize (IHbs a pos').
+           apply IHbs.
+           rewrite lookup_cons_ne_0 in H; auto.
+           rewrite H0 in H; simpl in *; auto.
+         }
+Qed.
+
+Theorem take_drop_txns:
+  forall (txn_id: nat) txns,
+    txn_id <= length txns ->
+    txn_upds txns = txn_upds (take txn_id txns) ++ txn_upds (drop txn_id txns).
+Proof.
+  induction txn_id.
+  - intros.
+    unfold txn_upds; simpl.
+    rewrite skipn_O; auto.
+  - intros. destruct txns.
+    + unfold txn_upds; simpl; auto.
+    + rewrite txn_upds_cons.
+      rewrite firstn_cons.
+      rewrite skipn_cons.
+      replace (txn_upds (p :: take txn_id txns)) with (txn_upds [p] ++ txn_upds (take txn_id txns)).
+      2: rewrite <- txn_upds_cons; auto.
+      rewrite <- app_assoc.
+      f_equal.
+      rewrite <- IHtxn_id; auto.
+      rewrite cons_length in H.
+      lia.
+Qed.
+
+Theorem updates_for_addr_app a l1 l2:
+  updates_for_addr a (l1 ++ l2) = updates_for_addr a l1 ++ updates_for_addr a l2.
+Proof.
+  unfold updates_for_addr.
+  rewrite <- fmap_app.
+  f_equal.
+  rewrite filter_app //.
+Qed.
+
+Theorem updates_since_to_last_disk σ a (txn_id : nat) installed :
+  wal_wf σ ->
+  disk_at_txn_id txn_id σ !! int.Z a = Some installed ->
+  (txn_id ≤ σ.(log_state.installed_lb))%nat ->
+  last_disk σ !! int.Z a = Some (latest_update installed (updates_since txn_id a σ)).
+Proof.
+  destruct σ.
+  unfold last_disk, updates_since, disk_at_txn_id.
+  simpl.
+  intros.
+  rewrite -> take_ge by lia.
+  rewrite (take_drop_txns (S txn_id) txns).
+  2: {
+    unfold wal_wf in H; intuition; simpl in *.
+    lia.
+  }
+  rewrite apply_upds_app.
+  generalize dependent H0.
+  generalize (apply_upds (txn_upds (take (S txn_id) txns)) d).
+  intros.
+  generalize (txn_upds (drop (S txn_id) txns)).
+  intros.
+  generalize dependent d0.
+  generalize dependent installed.
+  induction l; simpl; intros.
+  - auto.
+  - destruct a0. unfold updates_for_addr.
+    rewrite filter_cons; simpl.
+    destruct (decide (addr = a)); subst.
+    + simpl.
+      erewrite <- IHl.
+      { reflexivity. }
+      rewrite lookup_insert. auto.
+    + erewrite <- IHl.
+      { reflexivity. }
+      rewrite lookup_insert_ne; auto.
+      intro Hx. apply n. word.
+Qed.
